removed the bottom axiom

defs.v
@@ -104,7 +104,6 @@ Definition root_active t := ~(has_rnf t).
 Definition sim (U : term -> Prop) := par_clos (fun x y => U x /\ U y).
 
 Definition meaningless (U : term -> Prop) :=
-  U bot /\
   (forall x y, U x -> inf_beta x y -> U y) /\
   (forall x y n, U x -> U (x[n := y])) /\
   (forall x d c, U x -> U (shift d c x)) /\
