README.md
@@ -1,6 +1,5 @@
-
 This is a formalisation of coinductive confluence and normalisation
-proofs for the infinitary lambda-calculus. The following theorems are
+proofs for the infinitary lambda calculus. The following theorems are
 formalised.
 1. Confluence of Böhm reduction over any set of strongly meaningless
    terms.
@@ -12,5 +11,5 @@ formalised.
    meaningless terms.
 
 All basic definitions are in [defs.v](defs.v). The main results are in
-[main.v](main.v). Tested with Coq 8.7.1 and Coq 8.8.1. The compilation
-may take around 5-10 minutes.
+[main.v](main.v). Tested with Coq 8.7.1, Coq 8.8.1 and Coq 8.9. The
+compilation may take around 5-10 minutes.
